jar2bpl_test/regression/test_output/java_input.bpl
@@ -6,16 +6,19 @@ type boolArrHeap_type = [ref][int]bool;
 type refArrHeap_type = [ref][int]ref;
 type realArrHeap_type = [ref][int]int;
 type intArrHeap_type = [ref][int]int;
-const unique $null : ref;
 const unique $type : Field javaType;
 const unique $alloc : Field bool;
+const unique $null : ref;
 const { :sourceloc "Object.java",-1,-1,-1,-1 } unique java.lang.Object : javaType extends  complete;
-const { :sourceloc "InfeasibleCode01.java",-1,-1,-1,-1 } unique InfeasibleCode01 : javaType extends  unique java.lang.Object complete;
+const { :sourceloc "FalsePositives04.java",-1,-1,-1,-1 } unique FalsePositives04 : javaType extends  unique java.lang.Object complete;
 const { :sourceloc "Serializable.java",-1,-1,-1,-1 } unique java.io.Serializable : javaType extends  unique java.lang.Object complete;
+const { :sourceloc "Throwable.java",-1,-1,-1,-1 } unique java.lang.Throwable : javaType extends  unique java.io.Serializable, unique java.lang.Object complete;
+const { :sourceloc "Exception.java",-1,-1,-1,-1 } unique java.lang.Exception : javaType extends  unique java.lang.Throwable complete;
+const { :sourceloc "RuntimeException.java",-1,-1,-1,-1 } unique java.lang.RuntimeException : javaType extends  unique java.lang.Exception complete;
+const { :sourceloc "NullPointerException.java",-1,-1,-1,-1 } unique java.lang.NullPointerException : javaType extends  unique java.lang.RuntimeException complete;
 const { :sourceloc "Comparable.java",-1,-1,-1,-1 } unique java.lang.Comparable : javaType extends  unique java.lang.Object complete;
 const { :sourceloc "CharSequence.java",-1,-1,-1,-1 } unique java.lang.CharSequence : javaType extends  unique java.lang.Object complete;
-const { :sourceloc "String.java",-1,-1,-1,-1 } unique java.lang.String : javaType extends  unique java.lang.Comparable, unique java.lang.CharSequence, unique java.lang.Object, unique java.io.Serializable complete;
-const { :sourceloc "InfeasibleCode02.java",-1,-1,-1,-1 } unique InfeasibleCode02 : javaType extends  unique java.lang.Object complete;
+const { :sourceloc "String.java",-1,-1,-1,-1 } unique java.lang.String : javaType extends  unique java.io.Serializable, unique java.lang.CharSequence, unique java.lang.Comparable, unique java.lang.Object complete;
 var $heap : $heap_type;
 var $intArrayType : javaType;
 var $charArrayType : javaType;
@@ -28,8 +31,7 @@ var $boolArrHeap : boolArrHeap_type;
 var $refArrHeap : refArrHeap_type;
 var $realArrHeap : realArrHeap_type;
 var $intArrHeap : intArrHeap_type;
-var int$InfeasibleCode01$beginEndTag0 : Field int;
-var int$InfeasibleCode02$x0 : Field int;
+var java.lang.Object$FalsePositives04$first234 : Field ref;
 function $arrayType(t:javaType) returns ($ret:javaType);
 function $intToReal(x:int) returns ($ret:real);
 function $intToBool(x:int) returns ($ret:bool) { (if x == 0 then false else true) }
@@ -45,257 +47,129 @@ function $xorInt(x:int, y:int) returns ($ret:int);
 function $shlInt(x:int, y:int) returns ($ret:int);
 function $ushrInt(x:int, y:int) returns ($ret:int);
 function $shrInt(x:int, y:int) returns ($ret:int);
-procedure $new(obj_type:javaType) returns ($obj:ref);    ensures $obj != $null;    requires $heap[$obj,$alloc] == false;    ensures $heap[$obj,$type] == obj_type;    ensures $heap[$obj,$alloc] == true;    
+axiom (forall t : javaType :: $heap[$null,$type] <: t);
+procedure $new(obj_type:javaType) returns ($obj:ref);    ensures $heap[$obj,$type] == obj_type;    requires $heap[$obj,$alloc] == false;        ensures $obj != $null;    ensures $heap[$obj,$alloc] == true;
 
-procedure java.lang.Object$java.lang.Object$clone$43($this:ref) returns ($other:ref);    ensures $other != $null;    ensures $heap[$other,$type] == $heap[$this,$type];        ensures $heap[$other,$alloc] == true;
+procedure java.lang.Object$java.lang.Object$clone$43($this:ref) returns ($other:ref);        ensures $other != $null;    ensures $heap[$other,$alloc] == true;    ensures $heap[$other,$type] == $heap[$this,$type];
 
 procedure int$java.lang.String$compareTo$87($this:ref, $other:ref) returns ($return:int);    
 
-procedure void$InfeasibleCode01$infeasible08$1889($this:ref, $in_parameter__0:ref, $in_parameter__1:ref, $in_parameter__2:int) returns ($exception:ref);    
+procedure java.lang.Object$FalsePositives04$peekFirst$1890($this:ref) returns ($return:ref, $exception:ref);    modifies $heap;
 
-procedure int$java.lang.String$indexOf$102($this:ref, $in_parameter__0:ref, $in_parameter__1:int) returns ($return:int, $exception:ref);    
+procedure java.lang.Object$FalsePositives04$foo$1889($this:ref) returns ($return:ref, $exception:ref);    modifies $heap;
 
-procedure void$InfeasibleCode01$$la$init$ra$$1890($this:ref) returns ($exception:ref);    
+procedure java.lang.String$java.lang.Object$toString$44($this:ref) returns ($return:ref, $exception:ref);    
+
+procedure void$FalsePositives04$$la$init$ra$$1891($this:ref) returns ($exception:ref);    
 
 procedure void$java.lang.Object$$la$init$ra$$38($this:ref) returns ($exception:ref);    
 
-procedure void$InfeasibleCode02$infeasible01$2084($this:ref) returns ($exception:ref);    
-
-procedure void$InfeasibleCode02$infeasible07$2085($this:ref, $in_parameter__0:ref) returns ($exception:ref);    
-
-procedure void$InfeasibleCode02$$la$init$ra$$2086($this:ref) returns ($exception:ref);    
-
-implementation void$InfeasibleCode01$infeasible08$1889($this:ref, $in_parameter__0:ref, $in_parameter__1:ref, $in_parameter__2:int) returns ($exception:ref){
+implementation java.lang.Object$FalsePositives04$peekFirst$1890($this:ref) returns ($return:ref, $exception:ref){
     
-var searchString3 : ref;    
-var temp$412 : int;    
-var temp$513 : int;    
-var temp$311 : int;    
-var temp$614 : int;    
-var temp$816 : int;    
-var interncaret4 : int;    
-var source2 : ref;    
-var hitUp7 : int;    
-var flaghitup6 : int;    
-var temp$210 : int;    
-var temp$08 : int;    
-var temp$19 : int;    
-var temp$715 : int;    
-var temphitpoint5 : int;    
-var this1 : ref;
+var temp$24 : ref;    
+var this1 : ref;    
+var temp$35 : ref;    
+var temp$13 : ref;    
+var temp$68 : ref;    
+var temp$57 : ref;    
+var temp$79 : ref;    
+var temp$02 : ref;    
+var temp$46 : ref;
     assume $this != $null;
+    assume $heap[$return,$type] <: java.lang.Object;
+    assert { :sourceloc "FalsePositives04.java",8,5,17,5 } true;
     this1 := $this;
-    source2 := $in_parameter__0;
-    searchString3 := $in_parameter__1;
-    interncaret4 := $in_parameter__2;
-    temphitpoint5 := -1;
-    flaghitup6 := 0;
-    hitUp7 := 0;
   block1:
-    temp$08 := 0;
-    flaghitup6 := temp$08;
-    assert { :sourceloc "InfeasibleCode01.java",96,4,96,60 } source2 != $null;
-    call temp$19, $exception := int$java.lang.String$indexOf$102(source2, searchString3, interncaret4);
-    temphitpoint5 := temp$19;
-    if (temphitpoint5 > 0) {
-        assert { :sourceloc "InfeasibleCode01.java",97,7,97,22 } true;
+    assert { :sourceloc "FalsePositives04.java",8,5,17,5 } true;
+    assert { :sourceloc "FalsePositives04.java",10,18,10,22 } true;
+    call temp$02, $exception := java.lang.Object$FalsePositives04$foo$1889(this1);
+    if ($exception != $null && $heap[$exception,$type] <: java.lang.Throwable) {
         goto block2;
-    } else {
-        assert { :sourceloc "InfeasibleCode01.java",97,7,97,22 } true;
     }
-    goto block3;
-  block2:
-    assert { :sourceloc "InfeasibleCode01.java",97,42,97,52 } this1 != $null;
-    temp$210 := $heap[this1,int$InfeasibleCode01$beginEndTag0];
-    if (temphitpoint5 < temp$210) {
-        assert { :sourceloc "InfeasibleCode01.java",97,42,97,52 } true;
+    assert { :sourceloc "FalsePositives04.java",10,10,10,14 } true;
+    $heap := $heap[this1,java.lang.Object$FalsePositives04$first234 := temp$02];
+    assert { :sourceloc "FalsePositives04.java",11,20,11,24 } true;
+    temp$13 := $heap[this1,java.lang.Object$FalsePositives04$first234];
+    assert { :sourceloc "FalsePositives04.java",11,20,11,24 } true;
+    if (temp$13 != $null) {
+        assert { :sourceloc "FalsePositives04.java",11,20,11,24 } true;
+    } else {
+        assert { :noverify } true;
+        call $exception := $new(java.lang.NullPointerException);
+        goto block2;
+    }
+    call temp$24, $exception := java.lang.String$java.lang.Object$toString$44(temp$13);
+    if ($exception != $null && $heap[$exception,$type] <: java.lang.Throwable) {
+        goto block2;
+    }
+  block3:
+    assert { :sourceloc "FalsePositives04.java",11,20,11,24 } true;
+    assert { :sourceloc "FalsePositives04.java",13,14,13,18 } { :clone } true;
+    assert { :sourceloc "FalsePositives04.java",13,14,13,18 } { :clone } this1 != $null;
+    temp$35 := $heap[this1,java.lang.Object$FalsePositives04$first234];
+    assert { :sourceloc "FalsePositives04.java",13,14,13,18 } { :clone } true;
+    if (temp$35 == $null) {
+        assert { :sourceloc "FalsePositives04.java",13,14,13,18 } { :clone } true;
         goto block4;
     } else {
-        assert { :sourceloc "InfeasibleCode01.java",97,42,97,52 } true;
+        assert { :sourceloc "FalsePositives04.java",13,14,13,18 } { :clone } true;
     }
-    goto block3;
-    goto block4;
+    assert { :sourceloc "FalsePositives04.java",13,14,13,18 } { :clone } true;
+    goto block5;
   block4:
-    temp$311 := hitUp7;
-    temp$412 := temp$311 + 1;
-    hitUp7 := temp$412;
-    temp$513 := 1;
-    flaghitup6 := temp$513;
-    temp$614 := temphitpoint5;
-    temp$715 := $stringSizeHeap[searchString3];
-    temp$816 := temp$614 + temp$715;
-    interncaret4 := temp$816;
-  block3:
-    if (flaghitup6 == 0) {
-        assert { :sourceloc "InfeasibleCode01.java",103,11,103,19 } true;
-        goto block5;
-    } else {
-        assert { :sourceloc "InfeasibleCode01.java",103,11,103,19 } true;
-    }
-    goto block1;
+    assert { :sourceloc "FalsePositives04.java",13,14,13,18 } { :clone } true;
+    assert { :sourceloc "FalsePositives04.java",13,14,13,18 } { :clone } true;
+    temp$46 := $null;
+    assert { :sourceloc "FalsePositives04.java",14,11,14,22 } true;
+    $return := temp$46;
+    return;
   block5:
-    if (hitUp7 == 0) {
-        assert { :sourceloc "InfeasibleCode01.java",104,6,104,15 } true;
+    assert { :sourceloc "FalsePositives04.java",14,11,14,22 } true;
+    assert { :sourceloc "FalsePositives04.java",11,13,11,36 } true;
+    $return := temp$24;
+    return;
+  block2:
+    assert { :sourceloc "FalsePositives04.java",11,13,11,36 } true;
+    assert { :sourceloc "FalsePositives04.java",9,9,16,9 } true;
+    assert { :sourceloc "FalsePositives04.java",9,9,16,9 } $exception != $null;
+    assume $heap[$exception,$type] <: java.lang.Throwable;
+    temp$57 := $exception;
+    assert { :sourceloc "FalsePositives04.java",13,14,13,18 } { :clone } true;
+    assert { :sourceloc "FalsePositives04.java",13,14,13,18 } { :clone } this1 != $null;
+    temp$68 := $heap[this1,java.lang.Object$FalsePositives04$first234];
+    assert { :sourceloc "FalsePositives04.java",13,14,13,18 } { :clone } true;
+    if (temp$68 == $null) {
+        assert { :sourceloc "FalsePositives04.java",13,14,13,18 } { :clone } true;
         goto block6;
     } else {
-        assert { :sourceloc "InfeasibleCode01.java",104,6,104,15 } true;
+        assert { :sourceloc "FalsePositives04.java",13,14,13,18 } { :clone } true;
     }
+    assert { :sourceloc "FalsePositives04.java",13,14,13,18 } { :clone } true;
     goto block7;
   block6:
+    assert { :sourceloc "FalsePositives04.java",13,14,13,18 } { :clone } true;
+    assert { :sourceloc "FalsePositives04.java",13,14,13,18 } { :clone } true;
+    temp$79 := $null;
+    assert { :sourceloc "FalsePositives04.java",14,11,14,22 } true;
+    $return := temp$79;
+    return;
   block7:
+    assert { :sourceloc "FalsePositives04.java",14,11,14,22 } true;
+    assert { :sourceloc "FalsePositives04.java",14,11,14,22 } true;
+    $exception := temp$57;
     return;
 }
 
 
-implementation void$InfeasibleCode01$$la$init$ra$$1890($this:ref) returns ($exception:ref){
+implementation void$FalsePositives04$$la$init$ra$$1891($this:ref) returns ($exception:ref){
     
-var this17 : ref;
+var this10 : ref;
     assume $this != $null;
-    this17 := $this;
-    call $exception := void$java.lang.Object$$la$init$ra$$38(this17);
-    return;
-}
-
-
-implementation void$InfeasibleCode02$infeasible01$2084($this:ref) returns ($exception:ref){
-    
-var temp$122 : int;    
-var temp$223 : int;    
-var temp$324 : int;    
-var temp$425 : int;    
-var counter20 : int;    
-var hit19 : int;    
-var temp$021 : int;    
-var this18 : ref;
-    assume $this != $null;
-    this18 := $this;
-    hit19 := 0;
-    counter20 := 0;
-  block8:
-    temp$021 := 0;
-    hit19 := temp$021;
-    assert { :sourceloc "InfeasibleCode02.java",67,7,67,7 } this18 != $null;
-    temp$122 := $heap[this18,int$InfeasibleCode02$x0];
-    if (temp$122 == counter20) {
-        assert { :sourceloc "InfeasibleCode02.java",67,7,67,7 } true;
-        goto block9;
-    } else {
-        assert { :sourceloc "InfeasibleCode02.java",67,7,67,7 } true;
-    }
-    goto block10;
-  block9:
-    temp$223 := counter20;
-    temp$324 := temp$223 + 1;
-    counter20 := temp$324;
-    temp$425 := 1;
-    hit19 := temp$425;
-    if (counter20 > 10000) {
-        assert { :sourceloc "InfeasibleCode02.java",71,8,71,22 } true;
-        goto block11;
-    } else {
-        assert { :sourceloc "InfeasibleCode02.java",71,8,71,22 } true;
-    }
-    goto block12;
-  block11:
-    return;
-  block12:
-  block10:
-    if (hit19 == 0) {
-        assert { :sourceloc "InfeasibleCode02.java",76,11,76,13 } true;
-        goto block13;
-    } else {
-        assert { :sourceloc "InfeasibleCode02.java",76,11,76,13 } true;
-    }
-    goto block8;
-  block13:
-    return;
-}
-
-
-implementation void$InfeasibleCode02$infeasible07$2085($this:ref, $in_parameter__0:ref) returns ($exception:ref){
-    
-var temp$233 : ref;    
-var j30 : int;    
-var temp$738 : int;    
-var temp$637 : int;    
-var temp$334 : int;    
-var temp$031 : int;    
-var this26 : ref;    
-var temp$536 : int;    
-var temp$839 : int;    
-var end29 : int;    
-var temp27 : ref;    
-var temp$435 : int;    
-var repos28 : int;    
-var temp$940 : int;    
-var temp$132 : int;
-    assume $this != $null;
-    this26 := $this;
-    temp27 := $in_parameter__0;
-    repos28 := -1;
-    end29 := -1;
-    j30 := end29;
-  block14:
-    temp$031 := j30;
-    temp$132 := temp$031 + 1;
-    j30 := temp$132;
-    temp$233 := temp27;
-    temp$334 := j30;
-    assert { :sourceloc "InfeasibleCode02.java",85,7,85,18 } temp$334 < $arrSizeHeap[temp$233] && temp$334 >= 0;
-    temp$435 := $intArrHeap[temp$233][temp$334];
-    temp$536 := temp$435;
-    if (temp$536 == 97) {
-        assert { :sourceloc "InfeasibleCode02.java",85,7,85,18 } true;
-        goto block15;
-    } else {
-        assert { :sourceloc "InfeasibleCode02.java",85,7,85,18 } true;
-    }
-    goto block16;
-  block15:
-    temp$637 := j30 - end29;
-    temp$738 := temp$637 - 1;
-    repos28 := temp$738;
-  block16:
-    if (repos28 == -1) {
-        assert { :sourceloc "InfeasibleCode02.java",88,11,88,21 } true;
-        goto block17;
-    } else {
-        assert { :sourceloc "InfeasibleCode02.java",88,11,88,21 } true;
-    }
-    goto block18;
-  block17:
-    assert { :sourceloc "InfeasibleCode02.java",88,26,88,40 } temp27 != $null;
-    temp$839 := $arrSizeHeap[temp27];
-    if (j30 < temp$839) {
-        assert { :sourceloc "InfeasibleCode02.java",83,2,88,42 } true;
-        goto block14;
-    } else {
-        assert { :sourceloc "InfeasibleCode02.java",88,26,88,40 } true;
-    }
-    goto block18;
-    goto block14;
-  block18:
-    if (repos28 == -1) {
-        assert { :sourceloc "InfeasibleCode02.java",89,6,89,16 } true;
-        goto block19;
-    } else {
-        assert { :sourceloc "InfeasibleCode02.java",89,6,89,16 } true;
-    }
-    goto block20;
-  block19:
-    temp$940 := 0;
-    repos28 := temp$940;
-  block20:
-    return;
-}
-
-
-implementation void$InfeasibleCode02$$la$init$ra$$2086($this:ref) returns ($exception:ref){
-    
-var this41 : ref;
-    assume $this != $null;
-    this41 := $this;
-    call $exception := void$java.lang.Object$$la$init$ra$$38(this41);
+    assert { :sourceloc "FalsePositives04",3,-1,-1,-1 } true;
+    this10 := $this;
+    assert { :sourceloc "FalsePositives04",3,-1,-1,-1 } true;
+    call $exception := void$java.lang.Object$$la$init$ra$$38(this10);
+    assert { :sourceloc "FalsePositives04",3,-1,-1,-1 } true;
     return;
 }
 
